bedrock2/src/Word/Naive.v
@@ -3,6 +3,30 @@ Local Set Primitive Projections.
   
 Require Import Coq.ZArith.BinIntDef Coq.ZArith.BinInt.
 Require Import bedrock2.Word. Import word.
+Local Open Scope Z_scope.
+
+(* TODO: move me? *)
+(* from https://github.com/coq/coq/pull/8062/files#diff-c73fff6c197eb53a5ca574b51e21bf82 *)
+Require Import Lia.
+Module Z.  Lemma mod_0_r_ext x y : y = 0 -> x mod y = 0.
+  Proof. intro; subst; destruct x; reflexivity. Qed.
+  Lemma div_0_r_ext x y : y = 0 -> x / y = 0.
+  Proof. intro; subst; destruct x; reflexivity. Qed.
+
+  Ltac div_mod_to_quot_rem_generalize x y :=
+    pose proof (Z.div_mod x y);    pose proof (Z.mod_pos_bound x y);
+    pose proof (Z.mod_neg_bound x y);    pose proof (div_0_r_ext x y);
+    pose proof (mod_0_r_ext x y);    let q := fresh "q" in
+    let r := fresh "r" in    set (q := x / y) in *;
+    set (r := x mod y) in *;
+    clearbody q r.  Ltac div_mod_to_quot_rem_step :=
+    match goal with    | [ |- context[?x / ?y] ] => div_mod_to_quot_rem_generalize x y
+    | [ |- context[?x mod ?y] ] => div_mod_to_quot_rem_generalize x y    | [ H : context[?x / ?y] |- _ ] => div_mod_to_quot_rem_generalize x y
+    | [ H : context[?x mod ?y] |- _ ] => div_mod_to_quot_rem_generalize x y    end.
+  Ltac div_mod_to_quot_rem := repeat div_mod_to_quot_rem_step.
+End Z.
+Ltac mia := Z.div_mod_to_quot_rem; nia.
+
 
 (* TODO: move me? *)
 Definition minimize_eq_proof{A: Type}(eq_dec: forall (x y: A), {x = y} + {x <> y}){x y: A}    (pf: x = y): x = y :=
@@ -13,22 +37,25 @@ Definition minimize_eq_proof{A: Type}(eq_dec: forall (x y: A), {x = y} + {x <> y
 
 Section WithWidth.
   Context {width : Z}.
-  Let wrap_value z := Z.modulo z (Z.pow 2 width).
+  Let wrap_value z := z mod (2^width).
   Record rep := mk { unsigned : Z ; _ : wrap_value unsigned = unsigned }.
 
-  Context {width_nonneg : Z.le 0 width}.
+  Context {width_nonneg : Z.lt 0 width}.
 
   Lemma wrap_value_wrap_value z : wrap_value (wrap_value z) = wrap_value z.
     cbv [wrap_value]. rewrite Z.mod_mod. reflexivity.
-    eapply Z.pow_nonzero; [congruence | assumption].
+    eapply Z.pow_nonzero; [congruence | lia ].
   Qed.
 
   Definition wrap (z:Z) : rep :=
     mk (wrap_value z) (minimize_eq_proof Z.eq_dec (wrap_value_wrap_value z)).
+  Definition signed w :=
+    unsigned w mod 2^(width-1) - 2^(width-1) * (unsigned w / 2^(width-1)).
 
   Definition word : word.word width := {|
     word.rep := rep;
     word.unsigned := unsigned;
+    word.signed := signed;
     of_Z := wrap;
 
     add x y := wrap (Z.add (unsigned x) (unsigned y));
@@ -40,12 +67,20 @@ Section WithWidth.
     xor x y := wrap (Z.lxor (unsigned x) (unsigned y));
 
     mul x y := wrap (Z.mul (unsigned x) (unsigned y));
+    mulhss x y := wrap (Z.mul (signed x) (signed y) / 2^width);
+    mulhsu x y := wrap (Z.mul (signed x) (unsigned y) / 2^width);
+    mulhuu x y := wrap (Z.mul (unsigned x) (unsigned y) / 2^width);
+
+    divu x y := wrap (Z.div (unsigned x) (unsigned y));
+    divs x y := wrap (Z.div (signed x) (signed y));
 
     slu x y := wrap (Z.shiftl (unsigned x) (unsigned y));
     sru x y := wrap (Z.shiftr (unsigned x) (unsigned y));
+    srs x y := wrap (Z.shiftr (signed x) (unsigned y));
 
     eqb x y := Z.eqb (unsigned x) (unsigned y);
     ltu x y := Z.ltb (unsigned x) (unsigned y);
+    lts x y := Z.ltb (signed x) (signed y);
   |}.
 
   Lemma eq_unsigned {x y : rep} : unsigned x = unsigned y -> x = y.
@@ -58,8 +93,30 @@ Section WithWidth.
   Lemma of_Z_unsigned x : wrap (unsigned x) = x.
   Proof. eapply eq_unsigned; destruct x; cbn; assumption.  Qed.
 
+  Lemma signed_of_Z z : signed (wrap z) = wrap_value (z + 2 ^ (width - 1)) - 2 ^ (width - 1).
+  Proof.
+    cbv [unsigned signed wrap wrap_value].
+    set (M := 2 ^ (width - 1)).
+    assert (0 < M) by (change 0 with (2^(-1)); eapply Z.pow_lt_mono_r; lia).
+    assert (0 < 2*M) by lia.
+    replace (2^width) with (2*M) in * by
+        (subst M; rewrite <-Z.pow_succ_r, Z.sub_1_r, Z.succ_pred; nia).
+    clearbody M.
+    rewrite (Z.add_mod z M (2*M)) by lia.
+    assert (M/(2 * M)=0) as H2M by mia;
+      replace (M mod (2 * M)) with M by mia; clear H2M.
+    set (X := z mod (2*M));
+      destruct (ltac:(subst X; mia):(0 <= X < M \/ M <= X < 2*M)); clearbody X.
+    { assert (X/M = 0) by mia; assert ((X + M) / (2 * M) = 0); mia. }
+    { assert (X/M = 1) by mia; assert ((X + M) / (2 * M) = 1); mia. }
+  Qed.
+
+  Check fun (x y : word) => signed_of_Z (Z.shiftr (word.signed x) (word.unsigned y)).
+
   Lemma ok : word.ok word.
-  Proof. split; eauto using of_Z_unsigned. Qed.
+  Proof. split; eauto using of_Z_unsigned, signed_of_Z. Qed.
 End WithWidth.
 Arguments word : clear implicits.
 Arguments ok : clear implicits.
+
+Local Instance word8 : word.word 8 := word 8 ltac:(firstorder).
